Develop an alternative notion of equality

PartialMonad/CoroutineM/Equiv.lean
@@ -1,17 +1,160 @@
 import PartialMonad.CoroutineM.Get
+import Mathlib.Data.Set.Basic
+import Mathlib.Tactic.Relation.Trans
+
 
 namespace CoroutineM
 
 /-- Two coroutines are considered equivalent if both terminate and yield the same result,
 or if neither coroutine terminates -/
-inductive Equiv : CoroutineM α → CoroutineM α → Prop
-  | terminates {x y : CoroutineM α} :
-      (hx : x.Terminates) → (hy : y.Terminates) → x.run hx = y.run hy
-      → Equiv x y
-  | non_terminates {x y : CoroutineM α} : ¬x.Terminates → ¬y.Terminates → Equiv x y
+inductive Equiv (x y : CoroutineM α) : Prop
+  | terminates : (hx : x.Terminates) → (hy : y.Terminates) → x.run hx = y.run hy → Equiv x y
+  | non_terminates : ¬x.Terminates → ¬y.Terminates → Equiv x y
+
+-- inductive Bisim (x y : CoroutineM α) : Prop
+--   | mk
+--     (R : x.σ → y.σ → Prop)
+--     (state : R x.state y.state)
+--     (is_bisim : ∀ s₁ s₂, R s₁ s₂ → _)
+
+namespace Equiv
+
+/-! Show that `Equiv` is an equivalence relation -/
+section Equivalence
+
+theorem rfl (x : CoroutineM α) : Equiv x x := by
+  by_cases h : x.Terminates
+  · exact Equiv.terminates h h _root_.rfl
+  · exact Equiv.non_terminates h h
+
+theorem symm : Equiv x y → Equiv y x
+  | terminates hx hy run_eq => terminates hy hx run_eq.symm
+  | non_terminates hx hy => non_terminates hy hx
+
+theorem trans : Equiv x y → Equiv y z → Equiv x z
+  | terminates hx _ run_xy_eq,  terminates _ hz run_yz_eq => terminates hx hz (by simp_all)
+  | non_terminates hx _,        non_terminates _ hz       => non_terminates hx hz
+  | non_terminates ..,          terminates ..             => by contradiction
+
+def is_equivalence (α : Type u) : Equivalence (@Equiv α) := {refl := rfl, symm, trans}
+
+instance setoid (α : Type u) : Setoid (CoroutineM α) where
+  r := Equiv
+  iseqv := is_equivalence α
+
+instance : Trans (@Equiv α) (Equiv) (Equiv) := {trans}
+instance : Trans (@HasEquiv.Equiv (CoroutineM α) _) (HasEquiv.Equiv) (HasEquiv.Equiv) := {trans}
+
+end Equivalence
+
+/-- If a coroutine `x` terminates, yielding some value `a`, then `x` is equivalent to `pure a` -/
+theorem pure_run_equiv (x : CoroutineM α) (h : x.Terminates) :
+    pure (x.run h) ≈ x := by
+  apply terminates (pure_terminates _) h (run_pure _)
+
+theorem terminates_of_equiv {x y : CoroutineM α} (h_eqv : x ≈ y) :
+    x.Terminates → y.Terminates := by
+  intro h_terminates
+  cases h_eqv
+  · assumption
+  · contradiction
+
+-- theorem pure_equiv_iff {a : α} {x : CoroutineM α} :
+--     pure a ≈ x ↔ (∃ (h : x.Terminates), x.run h = a) := by
+--   sorry
+
+-- theorem iterate_bind_eq_of_iterate_x_eq
+
+@[simp] theorem bind_next_inl (x : CoroutineM α) (f : α → CoroutineM β) (s : x.σ) :
+    (x >>= f).next (.inl s) = .inl ((x.next s).map id (⟨·, (f _).state, (f _).next⟩)) := by
+  rfl
+
+@[simp] theorem nextState_mk {σ α} (next : σ → σ ⊕ α) (s : σ) :
+    nextState (mk next s) = (next s).map (mk next ·) id := by
+  rfl
+
+-- theorem iterate_bind_eq_of_x_iterate {x : CoroutineM α} {n} (h : (x.iterate n = .inl {})
+-- TODO: a theorem states that if `x.iterate n` has not yet completed, but is at new state `s'`,
+--       then `(x >>= f)` is at state `.inl s'`
+-- To phrase this nicely, we really need `iterate` to just return a state, rather than a full-blown
+-- coroutine
+
+theorem iterate_bind_isLeft_of {x : CoroutineM α} {n} (h : (x.iterate n).isLeft)
+    (f : α → CoroutineM β) : (iterate (x >>= f) n).isLeft := by
+  simp only [show (x >>= f) = {(x >>= f) with state := .inl x.state} from _root_.rfl]
+  simp only [show x = {x with state := x.state} from _root_.rfl] at h
+  generalize x.state = state at *
+  induction n generalizing state
+  case zero       => rfl
+  case succ n ih  => cases h' : x.next state <;> simp_all [iterate]
+
+theorem bind_iterate_minimumStepsToTerminate_x {x : CoroutineM α} (h : x.Terminates)
+    (f : α → CoroutineM β) :
+    (x >>= f).iterate (x.minimumStepsToTerminate h)
+    = let a := x.run h
+      .inl {(x >>= f) with state := .inr ⟨a, (f a).state, (f a).next⟩} := by
+  simp only
+  sorry
 
 
+/-- If `x` terminates, yielding some value `a`, then `x >>= f` is equivalent to `f a` -/
+theorem bind_equiv_of_terminates {x : CoroutineM α} (h : x.Terminates) :
+    (x >>= f) ≈ f (x.run h) := by
+  by_cases (f <| x.run h).Terminates
+  case pos h_f_terminates => sorry
+  case neg h_f_not_terminates =>
+    apply non_terminates _ h_f_not_terminates
+    sorry
 
-theorem pure_equiv (x : CoroutineM α) (∃ h, x.)
 
-end CoroutineM
+theorem non_terminates_of_cycle (x : CoroutineM α) (S : Set x.σ)
+    (h_state : x.state ∈ S)
+    (h_closed : ∀ s ∈ S, ∃ s' ∈ S, x.next s = .inl s') :
+    ¬x.Terminates := by
+  intro h_terminates
+  have iterate_mem_S : ∀ n, ∃ state ∈ S, x.iterate n = .inl {x with state} := by
+    intro n
+    induction n
+    case zero =>
+      simp; exact Exists.intro x.state ⟨h_state, _root_.rfl⟩
+    case succ n ih =>
+      rcases ih with ⟨s, s_mem_S, hs⟩
+      rcases h_closed _ s_mem_S with ⟨s', s'_mem, hs'⟩
+      simp [iterate_succ, hs, hs', s'_mem]
+  have ⟨s, _s_mem, hs⟩ := iterate_mem_S (x.minimumStepsToTerminate h_terminates)
+  have := x.iterate_minimumStepsToTerminate h_terminates
+  rw [hs] at this
+  contradiction
+
+-- theorem cycle_of_non_terminates {x : CoroutineM α} (h : ¬x.Terminates) :
+--   ∃ S, x.state ∈ S ∧ (∀ s ∈ S, ∃ s' ∈ S, x.next s = .inl s')
+
+theorem nextState_isLeft_of_iterate_succ_isLeft {x : CoroutineM α} :
+    (x.iterate (n+1)).isLeft → x.nextState.isLeft := by
+  unfold iterate; cases x.nextState <;> simp
+
+-- @[simp] theorem nextState_bind (x : CoroutineM α) (f : α → CoroutineM β) :
+--     nextState (x >>= f) = match nextState x with
+--       | .inl _ => .inl { x >>= f with state := _}
+--       | .inr _ => _ := by
+--   sorry
+
+theorem bind_non_terminates_of_left {x : CoroutineM α} (h : ¬x.Terminates) :
+    ¬(x >>= f).Terminates := by
+  simp only [Terminates, not_exists, Bool.not_eq_true, Sum.isRight_eq_false] at h ⊢
+  intro n
+  apply iterate_bind_isLeft_of (h n)
+
+theorem bind_equiv {x y : CoroutineM α} (f g : α → CoroutineM β) (hxy : x ≈ y)
+    (hfg : (h : x.Terminates) → (f <| x.run h) ≈ (g <| y.run <| terminates_of_equiv hxy h)) :
+    (x >>= f) ≈ (y >>= g) :=
+  match hxy with
+    | terminates hx hy _ =>
+        calc
+          x >>= f ≈ f (x.run hx)  := by apply bind_equiv_of_terminates
+                _ ≈ g (y.run hy)  := by apply hfg hx
+                _ ≈ y >>= g       := by apply Equiv.symm; apply bind_equiv_of_terminates
+    | non_terminates hx hy =>
+        non_terminates (bind_non_terminates_of_left hx) (bind_non_terminates_of_left hy)
+
+#print axioms bind_equiv
